new subtyping -- WARNING: not yet aligns with typechecking related stuff

tree/local.v
@@ -5,128 +5,672 @@ Require Import String List ZArith.
 Local Open Scope string_scope.
 Import ListNotations.
 Require Import Morphisms.
+Require Import Lia.
+
+(* 
+Class nlist (A: Type): Type :=
+{ under: list A;
+  uprop: under <> nil
+}.
+*)
+
+Inductive nlist (A : Type) : Type :=
+  | nnil : A -> nlist A
+  | ncons: A -> nlist A -> nlist A.
+
+Arguments nnil {_} _.
+Arguments ncons {_} _.
+
+Fixpoint nlength {A: Type} (l: nlist A): nat :=
+  match l with
+    | nnil x => S O
+    | ncons x xs => S (nlength xs)
+  end.
+
+Fixpoint nzip {A B: Type} (l1: nlist A) (l2: nlist B): nlist (A*B) :=
+  match (l1, l2) with
+    | (ncons x xs, ncons y ys) => ncons (x,y) (nzip xs ys) 
+    | (nnil x, nnil y)         => nnil (x,y)
+    | (nnil x, ncons y ys)     => nnil (x,y)
+    | (ncons x xs, nnil y)     => nnil (x,y)
+  end. 
+
+Inductive SSortedNList : list fin -> Prop :=
+  | sort1 : forall a, SSortedNList [a]
+  | sort2 : forall (z1 z2 : fin), forall l, le z1 z2 -> SSortedNList (z2 :: l) -> SSortedNList (z1 :: z2 :: l).
+
+Inductive nForall {A : Type} (P : A -> Prop) : nlist A -> Prop :=
+  | nForall_nil:  forall (x : A), P x -> nForall P (nnil x)
+  | nForall_cons : forall (x : A) (l : nlist A), P x -> nForall P l -> nForall P (ncons x l).
+
+Fixpoint nIn {A: Type} (a : A) (l : nlist A): Prop :=
+  match l with
+    | nnil a1     => a = a1
+    | ncons a1 xs => a = a1 \/ nIn a xs
+  end.
 
 (* local session trees *)
+(* CoInductive ltt: Type :=
+  | ltt_end : ltt
+  | ltt_recv: part -> list label -> list sort -> list ltt -> ltt
+  | ltt_send: part -> list label -> list sort -> list ltt -> ltt. *)
+
 CoInductive ltt: Type :=
   | ltt_end : ltt
-  | ltt_recv: part -> list (label*sort*ltt) -> ltt
-  | ltt_send: part -> list (label*sort*ltt) -> ltt.
+  | ltt_recv: part -> list (label*(sort*ltt)) -> ltt
+  | ltt_send: part -> list (label*(sort*ltt)) -> ltt. 
 
 Definition ltt_id (s: ltt): ltt :=
   match s with
     | ltt_end      => ltt_end
-    | ltt_recv p l => ltt_recv p l
+    | ltt_recv p l => ltt_recv p l 
     | ltt_send p l => ltt_send p l
   end.
 
 Lemma ltt_eq: forall s, s = ltt_id s.
 Proof. intro s; destruct s; easy. Defined.
 
-(* Inductive lttbisim (R: ltt -> ltt -> Prop): ltt -> ltt -> Prop :=
-  | lttbisim_end : lttbisim R ltt_end ltt_end
-  | lttbisim_recv: forall p l s xs ys,
-                   length xs = length ys ->
-                   List.Forall (fun u => R (fst u) (snd u)) (zip xs ys) ->
-                   lttbisim R (ltt_recv p (zip (zip l s) xs)) (ltt_recv p (zip (zip l s) ys)).
- *)
-Inductive lt2ltt (R: local -> ltt -> Prop): local -> ltt -> Prop :=
-  | lt2ltt_end: lt2ltt R l_end ltt_end
-  | lt2ltt_rcv: forall p l s xs ys,
-                length xs = length ys ->
-                List.Forall (fun u => R (fst u) (snd u)) (zip xs ys) ->
-                lt2ltt R (l_recv p (zip (zip l s) xs)) (ltt_recv p (zip (zip l s) ys))
-  | lt2ltt_snd: forall p l s xs ys,
-                length xs = length ys ->
-                List.Forall (fun u => R (fst u) (snd u)) (zip xs ys) ->
-                lt2ltt R (l_send p (zip (zip l s) xs)) (ltt_send p (zip (zip l s) ys))
-  | lt2ltt_mu : forall l t,
-                lt2ltt R (subst_local ((l_rec l) .: l_var) l) t ->
-                lt2ltt R (l_rec l) t.
+Definition nonE {A: Type} (l: list A): Prop :=
+  match l with
+    | [] => False
+    | x::xs => True
+  end.
 
-Definition lt2lttC l t := paco2 lt2ltt bot2 l t.
+Definition wfL {A: Type} (l: list A) := NoDup l /\ nonE l.
+
+Inductive wf (R: ltt -> Prop): ltt -> Prop :=
+  | wf_end : wf R ltt_end
+  | wf_recv: forall p l s t,
+             wfL l ->
+             length l = length s ->
+             length s = length t ->
+             Forall R t -> 
+             wf R (ltt_recv p (zip l (zip s t)))
+  | wf_send: forall p l s t,
+             wfL l ->
+             length l = length s ->
+             length s = length t ->
+             Forall R t ->
+             wf R (ltt_send p (zip l (zip s t))).
+
+Lemma mon_wf: monotone1 wf.
+Proof. unfold monotone1.
+       intros.
+       induction IN; intros.
+       - constructor.
+       - constructor. easy. easy. easy.
+         rewrite Forall_forall.
+         intros.
+         apply LE.
+         rewrite Forall_forall in H2.
+         apply H2. easy.
+       - constructor. easy. easy. easy.
+         rewrite Forall_forall.
+         intros.
+         apply LE.
+         rewrite Forall_forall in H2.
+         apply H2. easy.
+Qed.
+
+Definition wfC (t: ltt) := paco1 wf bot1 t.
+
+Class wfltt: Type :=
+{
+   utype: ltt;
+   sprop: wfC utype
+}.
+
+Fixpoint lkp (x: label) (l: list (label*(sort*ltt))): option(sort*ltt) :=
+  match l with
+    | []            => Datatypes.None
+    | (u,(v,t))::xs => if Nat.eqb x u then Datatypes.Some(v,t) else lkp x xs
+  end.
+
+
+Fixpoint wfrec (R1: sort -> sort -> Prop) (R2: ltt -> ltt -> Prop) (l1 l2: list (label*(sort*ltt))): Prop :=
+  match l1 with
+    | []              => True
+    | (l,(s',t'))::xs => 
+      let R := lkp l l2 in
+      match R with
+        | Datatypes.None      => False
+        | Datatypes.Some(s,t) => R1 s' s /\ R2 t t' /\ wfrec R1 R2 xs l2
+      end
+  end.
+
+Fixpoint wfsend (R1: sort -> sort -> Prop) (R2: ltt -> ltt -> Prop) (l1 l2: list (label*(sort*ltt))): Prop :=
+  match l1 with
+    | []              => True
+    | (l,(s,t))::xs => 
+      let R := lkp l l2 in
+      match R with
+        | Datatypes.None      => False
+        | Datatypes.Some(s',t') => R1 s s' /\ R2 t t' /\ wfsend R1 R2 xs l2
+      end
+  end.
 
 Inductive subtype (R: ltt -> ltt -> Prop): ltt -> ltt -> Prop :=
   | sub_end: subtype R ltt_end ltt_end
-  | sub_in : forall p l s' s xs ys,
-                    length s' = length s ->
-                    length xs = length ys ->
-                    List.Forall (fun u => subsort (fst u) (snd u)) (zip s' s) ->
-                    List.Forall (fun u => R (fst u) (snd u)) (zip xs ys) ->
-                    subtype R (ltt_recv p (zip (zip l s) xs)) (ltt_recv p (zip (zip l s') ys))
-  | sub_out: forall p l s' s xs ys,
-                    length s' = length s ->
-                    length xs = length ys ->
-                    List.Forall (fun u => subsort (fst u) (snd u)) (zip s s') ->
-                    List.Forall (fun u => R (fst u) (snd u)) (zip xs ys) ->
-                    subtype R (ltt_send p (zip (zip l s) xs)) (ltt_send p (zip (zip l s') ys)).
+  | sub_in : forall p xs ys,
+                    Nat.le (length ys) (length xs) ->
+                    wfrec subsort R ys xs ->
+                    subtype R (ltt_recv p xs) (ltt_recv p ys)
+  | sub_out : forall p xs ys,
+                     Nat.le (length xs) (length ys) ->
+                     wfsend subsort R xs ys ->
+                     subtype R (ltt_send p xs) (ltt_send p ys).
 
-Lemma destZip: forall {A B C: Type} (l: list (A * B * C)),
-               exists L S xs, l = (zip (zip L S) xs).
+Definition subtypeC l1 l2 := paco2 subtype bot2 l1 l2.
+
+Lemma destZip: forall {A B C: Type} (l: list (A * (B * C))),
+               exists L S xs, l = (zip L (zip S xs)).
 Proof. induction l; intros.
        - exists nil. exists nil. exists nil. easy.
        - destruct IHl as (L,(S,(xs,Hxs))).
-         destruct a as ((a1,a2),a3).
+         destruct a as (a1,(a2,a3)).
          simpl.
          exists (a1::L). exists (a2::S). exists(a3::xs).
          simpl. rewrite Hxs. easy.
 Qed.
 
-Lemma stReflH: forall R T, Reflexive R -> subtype R T T.
-Proof. intros.
-       case_eq T; intros.
-       - constructor.
-       - subst.
-         specialize (destZip l); intro Hdest.
-         destruct Hdest as (L,(S,(xs,Hxs))).
-         subst.
-         apply sub_in. easy. easy.
-         apply Forall_forall.
-         intros (x1,x2) Hx. simpl.
-         induction S; intros.
-         subst. simpl in Hx.
-         unfold In in Hx. easy.
-         subst. simpl in Hx.
-         destruct Hx as [Hx | Hx].
-         inversion Hx. apply srefl.
-         apply IHS. easy.
-         
-         apply Forall_forall.
-         intros (x1,x2) Hx. simpl.
-         induction xs; intros.
-         subst. simpl in Hx.
-         unfold In in Hx. easy.
-         subst. simpl in Hx.
-         destruct Hx as [Hx | Hx].
-         inversion Hx.
-         reflexivity.
-         apply IHxs. easy.
-
-         specialize (destZip l); intro Hdest.
-         destruct Hdest as (L,(S,(xs,Hxs))).
-         subst.
-         apply sub_out. easy. easy.
-         apply Forall_forall.
-         intros (x1,x2) Hx. simpl.
-         induction S; intros.
-         subst. simpl in Hx.
-         unfold In in Hx. easy.
-         subst. simpl in Hx.
-         destruct Hx as [Hx | Hx].
-         inversion Hx. apply srefl.
-         apply IHS. easy.
-
-         apply Forall_forall.
-         intros (x1,x2) Hx. simpl.
-         induction xs; intros.
-         subst. simpl in Hx.
-         unfold In in Hx. easy.
-         subst. simpl in Hx.
-         destruct Hx as [Hx | Hx].
-         inversion Hx. reflexivity.
-         apply IHxs. easy.
+Lemma ndestZip: forall {A B C: Type} (l: nlist (A * (B * C))),
+               exists L S xs, l = (nzip L (nzip S xs)).
+Proof. induction l; intros.
+       destruct a as (a1,(a2,a3)).
+       - exists (nnil a1). exists (nnil a2). exists (nnil a3). easy.
+       - destruct IHl as (L,(S,(xs,Hxs))).
+         destruct a as (a1,(a2,a3)).
+         simpl.
+         exists (ncons a1 L). exists (ncons a2 S). exists(ncons a3 xs).
+         simpl. rewrite Hxs. easy.
 Qed.
 
-Definition subtypeC l1 l2 := paco2 subtype bot2 l1 l2.
+Fixpoint unzipF {A B C: Type} (l: list(A*(B*C))): list A :=
+  match l with
+    | []            => []
+    | (u,(v,t))::xs => u::unzipF xs 
+  end.
+
+Lemma unzipIn: forall (l1:  list (label*(sort*ltt))) l s t, In (l, (s, t)) l1 -> In l (unzipF l1).
+Proof. intro l1.
+       induction l1; intros.
+       - simpl in *. easy.
+       - simpl in *.
+         destruct H, a, p.
+         inversion H. subst. simpl. left. easy.
+         simpl. right.
+         eapply IHl1. exact H.
+Qed.
+
+Lemma inDiff: forall {A: Type} (l: list A) a b, In a l -> ~In b l -> a <> b.
+Proof. intros A l.
+       induction l; intros.
+       - simpl in H. easy.
+       - simpl in *.
+         intro Ha.
+         destruct H. subst.
+         apply H0. left. easy.
+         subst.
+         apply H0. right. easy. 
+Qed.
+
+Lemma inLkp: forall (l1:  list (label*(sort*ltt))) l s t,
+  NoDup (unzipF l1) ->
+  In (l,(s,t)) l1 <-> lkp l l1 = Datatypes.Some(s, t).
+Proof. intro l1.
+       induction l1; intros.
+       split.
+       simpl. easy.
+       simpl. easy.
+       split.
+       intro Ha.
+       simpl.
+       destruct a, p.
+       simpl in Ha.
+       destruct Ha. inversion H0. subst.
+       rewrite Nat.eqb_refl. easy.
+       simpl in H.
+       pose proof H0 as H00.
+       apply unzipIn in H0.
+       inversion H. subst.
+       specialize(inDiff _ _ _ H0 H3); intros.
+       assert(Nat.eqb l n = false).
+       { rewrite Nat.eqb_neq. easy. }
+       rewrite H2.
+       apply IHl1. easy. easy.
+       intro Ha.
+       simpl in Ha.
+       destruct a, p. simpl.
+       case_eq(Nat.eqb l n); intros.
+       rewrite H0 in Ha.
+       rewrite Nat.eqb_eq in H0. subst.
+       inversion Ha. subst. left. easy.
+       rewrite H0 in Ha.
+       eapply IHl1 in Ha.
+       right. easy.
+       simpl in H.
+       inversion H. subst. easy.
+Qed.
+
+Lemma ninLkp: forall (l1:  list (label*(sort*ltt))) l,
+  NoDup (unzipF l1) ->
+  (forall s t, (~ In (l,(s,t)) l1)) <-> lkp l l1 = Datatypes.None.
+Proof. intro l1.
+       induction l1; intros.
+       - split. intro Ha.
+         simpl. easy.
+       - intro Ha.
+         simpl. easy.
+       - split. intro Ha.
+         simpl. destruct a, p.
+         simpl in Ha.
+         case_eq(Nat.eqb l n); intros.
+         rewrite Nat.eqb_eq in H0. subst.
+         specialize(Ha s l0).
+         destruct Ha. left. easy.
+         apply IHl1.
+         simpl in H. inversion H. subst. easy.
+         intros.
+         rewrite Nat.eqb_neq in H0.
+         intro Hb.
+         apply H0.
+         specialize(Ha s0 t).
+         destruct Ha. right. easy.
+         
+         intro Ha.
+         intros. simpl in Ha.
+         destruct a, p.
+         case_eq(Nat.eqb l n); intros.
+         rewrite Nat.eqb_eq in H0. subst.
+         rewrite Nat.eqb_refl in Ha.
+         easy.
+         rewrite H0 in Ha.
+         simpl.
+         intro Hb.
+         rewrite Nat.eqb_neq in H0.
+         apply H0.
+         destruct Hb.
+         inversion H1. easy.
+         apply IHl1 in H1. easy.
+         simpl in H. inversion H. easy.
+         easy.
+Qed.
+
+Lemma lkp_eq: forall l1 l2, 
+  NoDup (unzipF l1) ->
+  NoDup (unzipF l2) ->
+  (forall l, lkp l l1 = lkp l l2) <-> (forall x, In x l1 <-> In x l2).
+Proof. intros.
+       split. intros Ha (l,(s,t)).
+       case_eq(lkp l l1); case_eq(lkp l l2); intros.
+       - specialize(Ha l).
+         rewrite inLkp.
+         rewrite inLkp.
+         split.
+         intro Hb. rewrite <- Ha. easy.
+         intro Hb. rewrite Ha. easy.
+         easy. easy.
+         specialize(Ha l).
+         rewrite H1 in Ha.
+         rewrite H2 in Ha.
+         easy.
+         specialize(Ha l).
+         rewrite H1 in Ha.
+         rewrite H2 in Ha.
+         easy.
+         specialize(Ha l).
+         rewrite <- ninLkp in H1.
+         rewrite <- ninLkp in H2.
+         specialize(H1 s t).
+         specialize(H2 s t).
+         split; intro; easy.
+         easy. easy.
+         
+       intros.
+       case_eq(lkp l l1); case_eq(lkp l l2); intros.
+       destruct p, p0.
+       rewrite <- inLkp in H2.
+       rewrite <- inLkp in H3.
+       pose proof H1 as H10.
+       specialize(H1 (l, (s, l0))).
+       specialize(H10 (l, (s0, l3))).
+       apply H10 in H3.
+       rewrite inLkp in H3.
+       rewrite inLkp in H2.
+       rewrite H3 in H2.
+       inversion H2. subst. easy.
+       easy. easy. easy. easy.
+       
+       destruct p.
+       rewrite <- inLkp in H3.
+       rewrite <- ninLkp in H2.
+       specialize(H2 s l0). 
+       apply H1 in H3. easy.
+       easy. easy.
+       destruct p.
+       rewrite <- inLkp in H2.
+       rewrite <- ninLkp in H3.
+       specialize(H3 s l0). 
+       apply H1 in H2. easy.
+       easy. easy.
+       easy.
+Qed.
+
+Lemma helperL: forall (l1 l2:  list (label*(sort*ltt))) l (s: sort) (t: ltt) (R1: sort -> sort -> Prop) (R2: ltt -> ltt -> Prop),
+   Nat.le (length l1) (length l2) ->
+   wfrec R1 R2 l1 l2 ->
+   ( In (l,(s,t)) l1 ->
+     exists s' t', R1 s s' /\ R2 t' t /\ lkp l l2 = Datatypes.Some (s', t')
+   ).
+Proof. intro l1.
+       induction l1; intros.
+       - simpl in H1. easy.
+       - simpl in *.
+         destruct a as (l',(s',t')).
+         destruct H1.
+         inversion H1. subst.
+         case_eq(lkp l l2); intros.
+         + destruct p.
+           rewrite H2 in H0.
+           exists s0. exists l0. split; easy.
+         + rewrite H2 in H0. easy.
+           eapply IHl1. lia.
+           case_eq(lkp l' l2); intros.
+           rewrite H2 in H0. destruct p.
+           easy.
+           rewrite H2 in H0. easy.
+           easy.
+Qed.
+
+Lemma helperL2: forall (l1 l2:  list (label*(sort*ltt))) (R1: sort -> sort -> Prop) (R2: ltt -> ltt -> Prop),
+   Nat.le (length l1) (length l2) ->
+   ( forall l s t, In (l,(s,t)) l1 ->
+     exists s' t', R1 s s' /\ R2 t' t /\ lkp l l2 = Datatypes.Some (s', t')
+   ) -> wfrec R1 R2 l1 l2.
+Proof. intros.
+       revert l2 H H0.
+       induction l1; intros.
+       - simpl. easy.
+       - simpl.
+         destruct a as (l',(s',t')).
+         pose proof H0 as H00.
+         specialize(H0 l' s' t').
+         simpl in H0.
+         assert((l', (s', t')) = (l', (s', t')) \/ In (l', (s', t')) l1) by (left; easy).
+         specialize(H0 H1).
+         destruct H0 as (u,(v,(z,(Ha,Hb)))).
+         rewrite Hb.
+         split. easy. split. easy.
+         apply IHl1.
+         simpl in H. lia.
+         intros.
+         specialize(H00 l s t).
+         simpl in H00.
+         assert((l', (s', t')) = (l, (s, t)) \/ In (l, (s, t)) l1) by (right; easy).
+         specialize(H00 H2).
+         destruct H00 as (u1,(v1,(z1,(Ha1,Hb1)))).
+         exists u1. exists v1. split; easy.
+Qed.
+
+Lemma helperR: forall (l1 l2:  list (label*(sort*ltt))) l (s: sort) (t: ltt) (R1: sort -> sort -> Prop) (R2: ltt -> ltt -> Prop),
+   Nat.le (length l1) (length l2) ->
+   wfsend R1 R2 l1 l2 ->
+   ( In (l,(s,t)) l1 ->
+     exists s' t', R1 s s' /\ R2 t t' /\ lkp l l2 = Datatypes.Some (s', t')
+   ).
+Proof. intro l1.
+       induction l1; intros.
+       - simpl in H1. easy.
+       - simpl in *.
+         destruct a as (l',(s',t')).
+         destruct H1.
+         inversion H1. subst.
+         case_eq(lkp l l2); intros.
+         + destruct p.
+           rewrite H2 in H0.
+           exists s0. exists l0. split; easy.
+         + rewrite H2 in H0. easy.
+           eapply IHl1. lia.
+           case_eq(lkp l' l2); intros.
+           rewrite H2 in H0. destruct p.
+           easy.
+           rewrite H2 in H0. easy.
+           easy.
+Qed.
+
+
+Lemma helperR2: forall (l1 l2:  list (label*(sort*ltt))) (R1: sort -> sort -> Prop) (R2: ltt -> ltt -> Prop),
+   Nat.le (length l1) (length l2) ->
+   ( forall l s t, In (l,(s,t)) l1 ->
+     exists s' t', R1 s s' /\ R2 t t' /\ lkp l l2 = Datatypes.Some (s', t')
+   ) -> wfsend R1 R2 l1 l2.
+Proof. intros.
+       revert l2 H H0.
+       induction l1; intros.
+       - simpl. easy.
+       - simpl.
+         destruct a as (l',(s',t')).
+         pose proof H0 as H00.
+         specialize(H0 l' s' t').
+         simpl in H0.
+         assert((l', (s', t')) = (l', (s', t')) \/ In (l', (s', t')) l1) by (left; easy).
+         specialize(H0 H1).
+         destruct H0 as (u,(v,(z,(Ha,Hb)))).
+         rewrite Hb.
+         split. easy. split. easy.
+         apply IHl1.
+         simpl in H. lia.
+         intros.
+         specialize(H00 l s t).
+         simpl in H00.
+         assert((l', (s', t')) = (l, (s, t)) \/ In (l, (s, t)) l1) by (right; easy).
+         specialize(H00 H2).
+         destruct H00 as (u1,(v1,(z1,(Ha1,Hb1)))).
+         exists u1. exists v1. split; easy.
+Qed.
+
+Lemma refl_recv: forall (l1:  list (label*(sort*ltt))) (R1: sort -> sort -> Prop) (R2: ltt -> ltt -> Prop),
+   Reflexive R1 -> Reflexive R2 ->
+   NoDup(unzipF l1) ->
+   wfrec R1 R2 l1 l1.
+Proof. intros.
+       apply helperL2.
+       lia.
+       intros.
+       exists s. exists t.
+       split. easy. split. easy.
+       rewrite <- inLkp. easy.
+       easy.
+Qed.
+
+Lemma trans_recv: forall (l1 l2 l3:  list (label*(sort*ltt))) (R1: sort -> sort -> Prop) (R2: ltt -> ltt -> Prop),
+   Transitive R1 -> Transitive R2 ->
+   NoDup(unzipF l1) -> NoDup(unzipF l2) -> NoDup(unzipF l3) ->
+   Nat.le (length l1) (length l2) ->
+   Nat.le (length l2) (length l3) ->
+   wfrec R1 R2 l1 l2 -> wfrec R1 R2 l2 l3 -> wfrec R1 R2 l1 l3.
+Proof. intro l1.
+       induction l1; intros.
+       - simpl in H6. easy.
+       - destruct a as (l,(s,t)).
+         specialize(helperL ((l, (s, t)) :: l1) l2 l s t R1 R2 ); intro HH.
+         pose proof H6 as H60.
+         pose proof H7 as H70.
+         apply HH in H6.
+         destruct H6 as (s1,(t1,H6)).
+         specialize(helperL l2 l3 l s1 t1 R1 R2 ); intro HHH.
+         apply HHH in H7.
+         destruct H7 as (s2,(t2,H7)).
+         simpl.
+         destruct H7 as (H7a,(H7b,H7c)).
+         rewrite H7c.
+         split.
+         transitivity s1. easy. easy.
+         split.
+         transitivity t1. easy. easy.
+         eapply IHl1 with (l2 := l2).
+         easy. easy.
+         simpl in H1. inversion H1. easy.
+         easy. easy.
+         simpl in H4. lia.
+         easy.
+         simpl in H60.
+         destruct H6 as (H6a,(H6b,H6c)).
+         rewrite H6c in H60. easy.
+         easy. easy.
+         destruct H6 as (H6a,(H6b,H6c)).
+         rewrite inLkp.
+         easy.
+         easy.
+         simpl in H4. simpl. lia.
+         simpl. left. easy.
+Qed.
+
+Lemma refl_send: forall (l1:  list (label*(sort*ltt))) (R1: sort -> sort -> Prop) (R2: ltt -> ltt -> Prop),
+   Reflexive R1 -> Reflexive R2 ->
+   NoDup(unzipF l1) ->
+   wfsend R1 R2 l1 l1.
+Proof. intros.
+       apply helperR2.
+       lia.
+       intros.
+       exists s. exists t.
+       split. easy. split. easy.
+       rewrite <- inLkp. easy.
+       easy.
+Qed.
+
+Lemma trans_send: forall (l1 l2 l3:  list (label*(sort*ltt))) (R1: sort -> sort -> Prop) (R2: ltt -> ltt -> Prop),
+   Transitive R1 -> Transitive R2 ->
+   NoDup(unzipF l1) -> NoDup(unzipF l2) -> NoDup(unzipF l3) ->
+   Nat.le (length l1) (length l2) ->
+   Nat.le (length l2) (length l3) ->
+   wfsend R1 R2 l1 l2 -> wfsend R1 R2 l2 l3 -> wfsend R1 R2 l1 l3.
+Proof. intro l1.
+       induction l1; intros.
+       - simpl in H6. easy.
+       - destruct a as (l,(s,t)).
+         specialize(helperR ((l, (s, t)) :: l1) l2 l s t R1 R2 ); intro HH.
+         pose proof H6 as H60.
+         pose proof H7 as H70.
+         apply HH in H6.
+         destruct H6 as (s1,(t1,H6)).
+         specialize(helperR l2 l3 l s1 t1 R1 R2 ); intro HHH.
+         apply HHH in H7.
+         destruct H7 as (s2,(t2,H7)).
+         simpl.
+         destruct H7 as (H7a,(H7b,H7c)).
+         rewrite H7c.
+         split.
+         transitivity s1. easy. easy.
+         split.
+         transitivity t1. easy. easy.
+         eapply IHl1 with (l2 := l2).
+         easy. easy.
+         simpl in H1. inversion H1. easy.
+         easy. easy.
+         simpl in H4. lia.
+         easy.
+         simpl in H60.
+         destruct H6 as (H6a,(H6b,H6c)).
+         rewrite H6c in H60. easy.
+         easy. easy.
+         destruct H6 as (H6a,(H6b,H6c)).
+         rewrite inLkp.
+         easy.
+         easy.
+         simpl in H4. simpl. lia.
+         simpl. left. easy.
+Qed.
+
+Lemma unzipL: forall {A B C: Type} (l1: list A) (l2: list B) (l3: list C),
+  length l1 = length l2 ->
+  length l2 = length l3 ->
+  unzipF (zip l1 (zip l2 l3)) = l1.
+Proof. intros A B C l1.
+       induction l1; intros.
+       - simpl. case_eq l2; case_eq l3; intros.
+         + simpl. easy.
+         + simpl. easy.
+         + simpl. easy.
+         + simpl. easy.
+       - case_eq l2; case_eq l3; intros.
+         + simpl. subst. easy.
+         + simpl. subst. easy.
+         + simpl. subst. easy.
+         + simpl. f_equal.
+           apply IHl1.
+           subst. inversion H. easy.
+           subst. inversion H0. easy.
+Qed.
+
+Lemma transtH: forall t1 t2 t3 R,
+  Transitive R ->
+  wfC t1 ->
+  wfC t2 ->
+  wfC t3 ->
+  subtype R t1 t2 ->
+  subtype R t2 t3 ->
+  subtype R t1 t3.
+Proof. intros.
+       case_eq t1; case_eq t2; case_eq t3; intros; try (subst; simpl in *; easy).
+       subst.
+       inversion H3. subst.
+       inversion H4. subst.
+       constructor.
+       lia.
+       apply trans_recv with (l2 := l0).
+       repeat intro.
+       apply sstrans with (s2 := y). easy. easy.
+       easy. 
+       punfold H2.
+       inversion H2. subst.
+       unfold wfL in H7.
+       rewrite unzipL. easy. easy. easy.
+       apply mon_wf.
+       punfold H1.
+       inversion H1. subst.
+       unfold wfL in H7.
+       rewrite unzipL. easy. easy. easy.
+       apply mon_wf.
+       punfold H0.
+       inversion H0. subst.
+       unfold wfL in H7.
+       rewrite unzipL. easy. easy. easy.
+       apply mon_wf.
+       lia.
+       lia.
+       easy. easy.
+
+       subst.
+       inversion H3. subst.
+       inversion H4. subst.
+       constructor.
+       lia.
+       apply trans_send with (l2 := l0).
+       repeat intro.
+       apply sstrans with (s2 := y). easy. easy.
+       easy. 
+
+       punfold H0.
+       inversion H0. subst.
+       unfold wfL in H7.
+       rewrite unzipL. easy. easy. easy.
+       apply mon_wf.
+       punfold H1.
+       inversion H1. subst.
+       unfold wfL in H7.
+       rewrite unzipL. easy. easy. easy.
+       apply mon_wf.
+       punfold H2.
+       inversion H2. subst.
+       unfold wfL in H7.
+       rewrite unzipL. easy. easy. easy.
+       apply mon_wf.
+       lia.
+       lia.
+       easy. easy.
+Qed.
 
 Lemma st_mon: monotone2 subtype.
 Proof. unfold monotone2.
@@ -134,19 +678,37 @@ Proof. unfold monotone2.
        induction IN; intros.
        - constructor.
        - apply sub_in; try easy.
-         apply Forall_forall. 
-         intros (x0,x1) Ha.
-         rewrite Forall_forall in H2.
-         simpl. apply LE.
-         specialize(H2 (x0,x1)). simpl in H2.
-         now apply H2.
+         revert xs H H0.
+         induction ys; intros. easy.
+         destruct a as (l,(s,t)).
+         specialize(helperL ((l,(s,t)) :: ys) xs l s t subsort r); intro HH.
+         pose proof H0 as HN.
+         apply HH in H0.
+         destruct H0 as (s',(t',(Ha,(Hb,Hc)))).
+         simpl.
+         rewrite Hc.
+         split. easy. split. apply LE. easy.
+         apply IHys. simpl in H. lia.
+         simpl in HN. rewrite Hc in HN.
+         easy.
+         lia.
+         simpl. left. easy.
        - apply sub_out; try easy.
-         apply Forall_forall. 
-         intros (x0,x1) Ha.
-         rewrite Forall_forall in H2.
-         simpl. apply LE.
-         specialize(H2 (x0,x1)). simpl in H2.
-         now apply H2.
+         revert ys H H0.
+         induction xs; intros. easy.
+         destruct a as (l,(s,t)).
+         specialize(helperR ((l,(s,t)) :: xs) ys l s t subsort r); intro HH.
+         pose proof H0 as HN.
+         apply HH in H0.
+         destruct H0 as (s',(t',(Ha,(Hb,Hc)))).
+         simpl.
+         rewrite Hc.
+         split. easy. split. apply LE. easy.
+         apply IHxs. simpl in H. lia.
+         simpl in HN. rewrite Hc in HN.
+         easy.
+         lia.
+         simpl. left. easy.
 Qed.
 
 #[export]
